compcerto tactics

examples/BoundedQueueCode.v
@@ -175,11 +175,11 @@ Section CLIGHT.
       (Sreturn (Some (Etempvar rb_inc2_tmp tint))).
   Definition rb_inc2 : function :=
     {|
-      fn_return := tvoid;
+      fn_return := tint;
       fn_callconv := cc_default;
       fn_params := [];
       fn_vars := [];
-      fn_temps := [];
+      fn_temps := [ (rb_inc2_tmp, tint) ];
       fn_body := rb_inc2_body;
     |}.
   (* FIXME: *)
@@ -277,3 +277,101 @@ Section CLIGHT.
     |}.
 
 End CLIGHT.
+
+(** ** CompCertO Tactics *)
+Ltac crush_eval_expr :=
+  cbn;
+  lazymatch goal with
+  | [ |- eval_expr _ _ _ _ (Etempvar _ _) _ ] => apply eval_Etempvar; reflexivity
+  | [ |- eval_expr _ _ _ _ (Econst_int _ _) _ ] => apply eval_Econst_int
+  | [ |- eval_expr _ _ _ _ (Ebinop _ _ _ _) _ ] => eapply eval_Ebinop
+  | [ |- eval_expr _ _ _ _ (Evar _ _) _ ] => eapply eval_Elvalue
+  | [ |- eval_expr _ _ _ _ (Ederef _ _) _ ] => eapply eval_Elvalue
+  end.
+Ltac crush_eval_lvalue :=
+  cbn;
+  lazymatch goal with
+  | [ |- eval_lvalue _ _ _ _ (Evar _ _) _ _ ] =>
+      solve [ apply eval_Evar_local; reflexivity | apply eval_Evar_global; [ reflexivity | eassumption ] ]
+  | _ => constructor
+  end.
+Ltac crush_deref :=
+  cbn;
+  lazymatch goal with
+  | [ |- deref_loc (Tarray _ _ _) _ _ _ _] => eapply deref_loc_reference; reflexivity
+  | [ |- deref_loc (Tfunction _ _ _) _ _ _ _] => eapply deref_loc_reference; reflexivity
+  | [ |- deref_loc (Tint _ _ _) _ _ _ _] => eapply deref_loc_value; [ reflexivity | ]
+  end.
+
+Ltac crush_expr :=
+  repeat (cbn;
+    match goal with
+    | [ |- eval_expr _ _ _ _ _ _ ] => crush_eval_expr
+    | [ |- eval_lvalue _ _ _ _ _ _ _ ] => crush_eval_lvalue
+    | [ |- eval_exprlist _ _ _ _ _ _ _ ] => econstructor
+    | [ |- deref_loc _ _ _ _ _ ] => crush_deref
+    | [ |- Cop.sem_binary_operation _ _ _ _ _ _ _ = Some _] => try reflexivity
+    | [ |- Cop.sem_cast _ ?ty ?ty _ = Some _ ] => apply Cop.cast_val_casted; eauto
+    | [ |- assign_loc _ (Tint _ _ _) _ _ _ _ _ ] => eapply assign_loc_value; [ reflexivity | ]
+    | _ => try solve [ easy | eassumption ]
+    end).
+
+Ltac prove_norepet H :=
+  match type of H with
+  | False => inversion H
+  | (?a = ?b) \/ _ =>
+      destruct H as [H|H]; [inversion H|prove_norepet H]
+  end.
+
+Ltac solve_list_norepet :=
+  simpl;
+  match goal with
+  | |- list_norepet nil =>  apply list_norepet_nil
+  | |- list_norepet (?x :: ?l) =>
+      apply list_norepet_cons;
+      [simpl; let H := fresh "H" in intro H; prove_norepet H |solve_list_norepet]
+  end.
+Ltac destruct_or H :=
+  match type of H with
+  | _ \/ _ => destruct H as [H|H]; [ |destruct_or H]
+  | _ => idtac
+  end.
+
+Ltac solve_list_disjoint :=
+  simpl; unfold list_disjoint; simpl; red;
+  let x := fresh "x" in
+  let y := fresh "y" in
+  let Lx := fresh "Lx" in
+  let Ly := fresh "Ly" in
+  let xyEq := fresh "xyEq" in
+  intros x y Lx Ly xyEq; try rewrite xyEq in *; clear xyEq;
+  destruct_or Lx; destruct_or Ly; subst; try solve [inversion Lx]; try solve [inversion Ly].
+
+Ltac crush_step := cbn;
+  match goal with
+  | [ |- Step _ (Callstate _ _ _ _) _ _ ] =>
+      eapply step_internal_function;
+      [ eauto | constructor; cbn;
+                [ solve_list_norepet
+                | solve_list_norepet
+                | solve_list_disjoint
+                | repeat (econstructor; simpl; auto)
+                | reflexivity ] ]
+  | [ |- Step _ (State _ (Ssequence _ _) _ _ _ _) _ _ ] => apply step_seq
+  | [ |- Step _ (State _ (Sset _ _) _ _ _ _) _ _ ] => apply step_set
+  | [ |- Step _ (State _ (Scall _ _ _) _ _ _ _) _ _ ] => eapply step_call
+  | [ |- Step _ (Returnstate _ _ _) _ _ ] => eapply step_returnstate
+  | [ |- Step _ (State _ Sskip (Kseq _ _) _ _ _) _ _ ] => apply step_skip_seq
+  | [ |- Step _ (State _ (Sassign _ _) _ _ _ _) _ _ ] => eapply step_assign
+  | [ |- Step _ (State _ (Sreturn None) _ _ _ _) _ _ ] => eapply step_return_0
+  | [ |- Step _ (State _ (Sreturn (Some _)) _ _ _ _) _ _ ] => eapply step_return_1
+  | [ |- Step _ (State _ ?s _ _ _ _) _ _ ] => is_const s; unfold s; crush_step
+  end.
+
+Ltac lts_step := eapply star_left with (t1 := E0) (t2 := E0); [ | | reflexivity ].
+
+Ltac crush_star :=
+  match goal with
+  | [ |- Star _ (Returnstate _ Kstop _) _ _ ] => eapply star_refl
+  | _ => lts_step; [ crush_step; crush_expr | cbn; try crush_star ]
+  end.
