examples/BoundedQueueProof.v
@@ -1,0 +1,960 @@
+From Coq Require Import Lia.
+From models Require Import
+     IntSpec.
+From examples Require Import
+     CAL CompCertIntSpec RefConv
+     CompCertCAL BoundedQueueCode.
+From lattices Require Import
+     Upset Downset FCD.
+From structures Require Import Lattice. (* subrel *)
+From compcert Require Import
+     Integers Maps Coqlib
+     Memory AST Values
+     Clight Ctypes
+     LanguageInterface
+     Events Globalenvs
+     Smallstep.
+
+Import ListNotations ISpec.
+
+(** * Example: ring buffer and bounded queue *)
+
+Parameter cal_val_rel: CAL.val -> val -> Prop.
+Hypothesis val_is_int:
+  forall c v, cal_val_rel c v -> Cop.val_casted v tint.
+Hint Resolve val_is_int.
+
+Section MARSHALL.
+
+  Inductive cal_nat_rel: nat -> val -> Prop :=
+  | cal_nat_rel_intro n i:
+    Z.of_nat n = Integers.Int.intval i ->
+    cal_nat_rel n (Vint i).
+  Inductive cal_void_rel: unit -> val -> Prop :=
+  | cal_void_rel_intro: cal_void_rel tt Vundef.
+
+  Context (se: Genv.symtbl).
+
+  (** Refinement Conventions *)
+  Inductive rb_rc_rel: rc_rel rb_sig c_esig :=
+  | rb_set_rel i v vf sg c_i c_v b R:
+    vf = Vptr b Integers.Ptrofs.zero ->
+    Genv.find_symbol se set_id = Some b ->
+    c_i = Vint (Integers.Int.repr (Z.of_nat i)) ->
+    cal_val_rel v c_v ->
+    subrel cal_void_rel R ->
+    sg = set_sg ->
+    rb_rc_rel _ (set i v) _ (c_event vf sg [ c_i ; c_v ]) R
+  | rb_get_rel i vf sg c_i b R:
+    vf = Vptr b Integers.Ptrofs.zero ->
+    Genv.find_symbol se get_id = Some b ->
+    c_i = Vint (Integers.Int.repr (Z.of_nat i)) ->
+    subrel cal_val_rel R ->
+    sg = get_sg ->
+    rb_rc_rel _ (CAL.get i) _ (c_event vf sg [ c_i ]) R
+  | rb_inc1_rel vf sg b R:
+    vf = Vptr b Integers.Ptrofs.zero ->
+    Genv.find_symbol se inc1_id = Some b ->
+    subrel cal_nat_rel R ->
+    sg = inc1_sg ->
+    rb_rc_rel _ inc1 _ (c_event vf sg [ ]) R
+  | rb_inc2_rel vf sg b R:
+    vf = Vptr b Integers.Ptrofs.zero ->
+    Genv.find_symbol se inc2_id = Some b ->
+    subrel cal_nat_rel R ->
+    sg = inc2_sg ->
+    rb_rc_rel _ inc2 _ (c_event vf sg [ ]) R.
+
+  Inductive bq_rc_rel: rc_rel bq_sig c_esig :=
+  | bq_enq_rel v vf sg c_v b R:
+    vf = Vptr b Integers.Ptrofs.zero ->
+    Genv.find_symbol se enq_id = Some b ->
+    cal_val_rel v c_v ->
+    subrel cal_void_rel R ->
+    sg = enq_sg ->
+    bq_rc_rel _ (enq v) _ (c_event vf sg [ c_v ]) R
+  | bq_deq_rel vf sg b R:
+    vf = Vptr b Integers.Ptrofs.zero ->
+    Genv.find_symbol se deq_id = Some b ->
+    subrel cal_val_rel R ->
+    sg = deq_sg ->
+    bq_rc_rel _ deq _ (c_event vf sg [ ]) R.
+
+  Program Definition rb_rc : rb_sig <=> c_esig :=
+    {|
+      refconv_rel := rb_rc_rel;
+    |}.
+  Next Obligation.
+    intros * x y Hxy H.
+    destruct H; econstructor; eauto; etransitivity; eauto.
+  Qed.
+
+  Program Definition bq_rc : bq_sig <=> c_esig :=
+    {|
+      refconv_rel := bq_rc_rel;
+    |}.
+  Next Obligation.
+    intros * x y Hxy H.
+    destruct H; econstructor; eauto; etransitivity; eauto.
+  Qed.
+
+End MARSHALL.
+
+(* TODO: develop handy tactics *)
+Tactic Notation "inf_intro" ident(x) :=
+  unfold finf; rewrite !Inf.mor; apply inf_iff ; intro x; cbn.
+
+Tactic Notation "sup_intro" ident(x) :=
+  unfold fsup; rewrite !Inf.mor; apply sup_iff ; intro x; cbn.
+
+Ltac sup_at x :=
+  unfold fsup; rewrite !Sup.mor; eapply (sup_at x); cbn.
+
+Ltac inf_at x :=
+  unfold finf; rewrite !Sup.mor; eapply (inf_at x); cbn.
+
+Lemma type_pair_des:
+  forall a b c d, (a * c)%type = (b * d)%type -> a = b /\ c = d.
+Proof. Admitted.
+
+Import Ptrofs.
+
+Lemma genv_funct_symbol se id b f (p: Clight.program):
+  Genv.find_symbol se id = Some b ->
+  (prog_defmap p) ! id = Some (Gfun f) ->
+  Genv.find_funct (Clight.globalenv se p) (Vptr b zero) = Some f.
+Proof.
+  intros H1 H2.
+  unfold Genv.find_funct, Genv.find_funct_ptr.
+  destruct eq_dec; try congruence.
+  apply Genv.find_invert_symbol in H1. cbn.
+  rewrite Genv.find_def_spec. rewrite H1.
+  rewrite H2. reflexivity.
+Qed.
+
+Section RB.
+  Open Scope Z_scope.
+  Context (se:Genv.symtbl).
+
+  Lemma find_set b:
+    Genv.find_symbol se set_id = Some b ->
+    Genv.find_funct (Clight.globalenv se rb_program) (Vptr b zero) = Some (Internal rb_set).
+  Proof. intros. eapply genv_funct_symbol; eauto. Qed.
+
+  Lemma find_get b:
+    Genv.find_symbol se get_id = Some b ->
+    Genv.find_funct (Clight.globalenv se rb_program) (Vptr b zero) = Some (Internal rb_get).
+  Proof. intros. eapply genv_funct_symbol; eauto. Qed.
+
+  Lemma find_inc1 b:
+    Genv.find_symbol se inc1_id = Some b ->
+    Genv.find_funct (Clight.globalenv se rb_program) (Vptr b zero) = Some (Internal rb_inc1).
+  Proof. intros. eapply genv_funct_symbol; eauto. Qed.
+
+  Lemma find_inc2 b:
+    Genv.find_symbol se inc2_id = Some b ->
+    Genv.find_funct (Clight.globalenv se rb_program) (Vptr b zero) = Some (Internal rb_inc2).
+  Proof. intros. eapply genv_funct_symbol; eauto. Qed.
+
+  Hint Resolve find_get find_set find_inc1 find_inc2.
+
+  Inductive R_cnt (id: positive): nat -> mem -> Prop :=
+  | R_cnt_intro b v n m:
+    Genv.find_symbol se id = Some b ->
+    Mem.load Mint32 m b 0 = Some v ->
+    cal_nat_rel n v -> (n < CAL.N)%nat ->
+    Mem.range_perm m b 0 4 Cur Writable ->
+    R_cnt id n m.
+
+  Inductive R_arr : (nat -> CAL.val) -> mem -> Prop :=
+  | R_arr_intro f b m:
+    Genv.find_symbol se arr_id = Some b ->
+    (forall i, exists v, Mem.load Mint32 m b (4 * Z.of_nat i) = Some v /\
+                 cal_val_rel (f i) v) ->
+    (forall ofs, 0 <= ofs < 4 * Nz + 4 ->
+            Mem.perm m b ofs Cur Writable) ->
+    R_arr f m.
+
+  Inductive R_rb: rb_state -> mem -> Prop :=
+  | R_rb_intro f c1 c2 m:
+    R_cnt cnt1_id c1 m -> R_cnt cnt2_id c2 m -> R_arr f m ->
+    Ple (Genv.genv_next se) (Mem.nextblock m) ->
+    R_rb (f, c1, c2) m.
+
+  Hypothesis se_valid: Genv.valid_for (erase_program bq_program) se.
+
+  Hypothesis Nbound : 4 * Nz <= max_unsigned.
+  Hypothesis Nbound' : 4 * Nz <= Int.max_unsigned.
+  Hypothesis N_neq_0: Nz <> 0.
+
+  Lemma cnt_inc_simp c i:
+    Z.of_nat c = Int.intval i -> (c < CAL.N)%nat ->
+    Z.of_nat (S c mod CAL.N) = Int.intval (Int.modu (Int.add i (Int.repr 1)) (Int.repr Nz)).
+  Proof.
+    intros H1 H2. unfold Int.add, Int.modu.
+    apply inj_le in H2. rewrite Nat2Z.inj_succ in H2.
+    rewrite H1 in H2.
+    repeat rewrite Int.unsigned_repr.
+    all: unfold Nz in *; cbn -[Z.mul] in *; unfold Int.unsigned; try lia.
+    - unfold Int.unsigned. rewrite <- H1.
+      rewrite mod_Zmod.
+      + f_equal. rewrite Nat2Z.inj_succ. reflexivity.
+      + lia.
+    - unfold Int.unsigned. rewrite <- H1.
+      exploit (Z.mod_pos_bound (Z.of_nat c + 1) (Z.of_nat CAL.N)); lia.
+  Qed.
+
+  Lemma rb_code_correct:
+    L_rb [= (right_arrow (rb_rc se * rel_rc R_rb)%rc)
+         @ (right_arrow c_rc)
+         @ ang_lts_spec (semantics2 rb_program se) @ bot.
+  Proof.
+    intros ? [? ? m [ s ]]. destruct s as [ [ f c1 ] c2 ].
+    Local Opaque semantics2.
+    unfold compose. cbn. unfold rc_adj_right. cbn.
+    inf_intro ar. inf_intro x. destruct x as [ ? ? c_m [ mm ] ].
+    destruct c_m as [vf sg args].
+    inf_intro x. destruct x as [ Rp Hr ]. cbn.
+    intm. inf_intro ar'. inf_intro q. destruct q as [ q ].
+    inf_intro x. destruct x as [ Rc Hc ]. cbn.
+    intm. simple inversion Hc. intros. depsubst.
+    inv H3. inv H5. clear Hc H2 H4. rename H1 into HRc.
+    simple inversion Hr.
+    apply type_pair_des in H2. inv H2.
+    apply type_pair_des in H4. inv H4.
+    depsubst. inv H3. inv H5.
+    depsubst. cbn. intros HRev HRst HRp.
+    simple inversion HRst. depsubst. clear H1 H3 Hr. inv H2. inv H4.
+    clear HRst. intros HRst HRx.
+    unfold fsup. setoid_rewrite Sup.mor.
+    setoid_rewrite FCD.ext_ana. cbn.
+    rewrite <- Sup.mor.
+    simple inversion HRev; intros; depsubst; clear HRev.
+    (* set *)
+    - clear H7. inv H8.
+      apply assert_l. intros Hi. apply inj_lt in Hi.
+      rename H0 into Hb. rename H2 into Hv. rename H3 into HRr.
+      setoid_rewrite sup_sup. rewrite !Sup.mor.
+      (* initial_state *)
+      eapply (sup_at (exist _ _ _)); cbn. Unshelve.
+      3: { cbn. repeat econstructor; eauto. inv HRst. eauto. }
+      cbn. rewrite lts_spec_step.
+      rewrite !Sup.mor_join. apply join_l. apply join_l.
+      unfold fsup. rewrite !Sup.mor.
+      (* internal steps *)
+      inv HRst. inv H5. rename mm into m.
+      edestruct (Mem.valid_access_store m Mint32 b0 (4 * Z.of_nat i)) as (m' & Hm').
+      {
+        constructor.
+        - intros ofs Hofs. apply H1. unfold Nz. split.
+          lia. cbn [size_chunk] in Hofs. lia.
+        - apply Z.divide_factor_l.
+      }
+      eapply (sup_at (exist _ _ _)); cbn. Unshelve.
+      4: {
+        cbn. crush_star.
+        match goal with
+        | [ H: Mem.store _ ?m ?b ?ofs ?v = Some ?m' |- Mem.store _ ?m ?b ?ofs' ?v' = Some _ ] =>
+            replace ofs' with ofs; [ apply H | ]
+        end.
+        rewrite add_zero_l.
+        unfold of_intu, of_int, mul.
+        rewrite Int.unsigned_repr.
+        repeat rewrite unsigned_repr.
+        all: unfold Nz in *; try lia.
+      }
+      (* final step *)
+      rewrite lts_spec_step. rewrite !Sup.mor_join.
+      apply join_r. unfold fsup.
+      rewrite !Sup.mor. eapply (sup_at (exist _ _ _)); cbn.
+      Unshelve. 3: { cbn. econstructor. } cbn.
+      (* re-establish the relation *)
+      setoid_rewrite FCD.ext_ana. cbn.
+      setoid_rewrite FCD.ext_ana. cbn.
+      rewrite !Sup.mor.
+      eapply (sup_at (exist _ (Vundef, m') _)); cbn. Unshelve.
+      2: { cbn. apply HRc. reflexivity. } cbn.
+      setoid_rewrite FCD.ext_ana. cbn.
+      eapply (sup_at (exist _ (tt, (update f i v, c1, c2)) _)). Unshelve.
+      2: {
+        cbn. apply HRp. split.
+        - now apply HRr.
+        - apply HRx. cbn. constructor.
+          + destruct H2. econstructor; eauto.
+            erewrite Mem.load_store_other; eauto.
+            left. intros Hbb. subst.
+            exploit Genv.find_symbol_injective. apply H2. apply H.
+            intros. easy.
+            intros ofs Hofs. eapply Mem.perm_store_1; eauto.
+          + destruct H3. econstructor; eauto.
+            erewrite Mem.load_store_other; eauto.
+            left. intros Hbb. subst.
+            exploit Genv.find_symbol_injective. apply H3. apply H.
+            intros. easy.
+            intros ofs Hofs. eapply Mem.perm_store_1; eauto.
+          + econstructor; eauto. intros ix.
+            * unfold update in *. destruct Nat.eq_dec.
+              -- subst. exists c_v. split; auto.
+                 erewrite Mem.load_store_same; eauto.
+                 f_equal.
+                 eapply SimplLocalsproof.val_casted_load_result.
+                 eapply val_is_int; eauto. reflexivity.
+              -- edestruct (H0 ix) as (vx & Hvx & Hrv).
+                 exists vx; split; auto.
+                 erewrite Mem.load_store_other; eauto. right.
+                 apply not_eq in n. destruct n.
+                 ++ right. apply inj_lt in H4. cbn [size_chunk]. lia.
+                 ++ left. apply inj_lt in H4. cbn [size_chunk]. lia.
+            * intros ofs Hofs. eapply Mem.perm_store_1; eauto.
+          + erewrite Mem.nextblock_store; eauto.
+      } cbn. reflexivity.
+    (* get *)
+    - clear H6. inv H7.
+      apply assert_l. intros Hi.
+      rename H0 into Hb. rename H2 into HRr.
+      setoid_rewrite sup_sup. rewrite !Sup.mor.
+      (* initial_state *)
+      eapply (sup_at (exist _ _ _)); cbn. Unshelve.
+      3: { cbn. repeat econstructor; eauto. inv HRst. eauto. }
+      rewrite lts_spec_step.
+      rewrite !Sup.mor_join. apply join_l. apply join_l.
+      unfold fsup. rewrite !Sup.mor.
+      (* internal steps *)
+      inv HRst. inv H5. rename mm into m.
+      edestruct (H0 i) as (vx & Hvx & Hvr).
+      eapply (sup_at (exist _ _ _)); cbn. Unshelve.
+      3: {
+        cbn. crush_star.
+        match goal with
+        | [ H: Mem.load _ ?m ?b ?ofs = Some _ |- Mem.load _ ?m ?b ?ofs' = Some _ ] =>
+            replace ofs' with ofs; [ apply H | ]
+        end.
+        unfold of_intu, of_int, mul.
+        rewrite add_zero_l.
+        rewrite Int.unsigned_repr.
+        repeat rewrite unsigned_repr.
+        all: unfold Nz in *; try lia.
+      }
+      (* final state *)
+      rewrite lts_spec_step. rewrite !Sup.mor_join.
+      apply join_r. unfold fsup.
+      rewrite !Sup.mor. eapply (sup_at (exist _ _ _)); cbn.
+      Unshelve. 3: { cbn. econstructor. } cbn.
+      (* re-establish the relation *)
+      setoid_rewrite FCD.ext_ana. cbn.
+      setoid_rewrite FCD.ext_ana. cbn.
+      rewrite !Sup.mor.
+      eapply (sup_at (exist _ (vx, m) _)); cbn. Unshelve.
+      2: { cbn. apply HRc. reflexivity. } cbn.
+      setoid_rewrite FCD.ext_ana. cbn.
+      eapply (sup_at (exist _ (f i, (f, c1, c2)) _)); cbn.
+      Unshelve.
+      2: {
+        cbn. apply HRp. split; eauto.
+        apply HRx. cbn. constructor; eauto.
+        econstructor; eauto.
+      }
+      reflexivity.
+    (* inc1 *)
+    - clear H5. inv H6.
+      rename H0 into Hb. rename H1 into HR1.
+      setoid_rewrite sup_sup. rewrite !Sup.mor.
+      (* initial_state *)
+      eapply (sup_at (exist _ _ _)); cbn. Unshelve.
+      3: { cbn. repeat econstructor; eauto. inv HRst; eauto. }
+      rewrite lts_spec_step.
+      rewrite !Sup.mor_join. apply join_l. apply join_l.
+      unfold fsup. rewrite !Sup.mor.
+      inv HRst. inv H2.
+      (* internal steps *)
+      inv H1. rename mm into m.
+      edestruct (Mem.valid_access_store m Mint32 b0 0) as (m' & Hm').
+      {
+        constructor.
+        - intros ofs Hofs. apply H7. cbn [size_chunk] in Hofs. lia.
+        - apply Z.divide_0_r.
+      }
+      edestruct (Mem.valid_access_store m' Mint32 b0 0) as (m'' & Hm'').
+      {
+        constructor.
+        - intros ofs Hofs. eapply Mem.perm_store_1; eauto.
+        - apply Z.divide_0_r.
+      }
+      eapply (sup_at (exist _ _ _)); cbn. Unshelve.
+      5: {
+        cbn.
+        do 7 (lts_step; [ crush_step; crush_expr | ]). now constructor.
+        do 2 (lts_step; [ crush_step; crush_expr | ]). erewrite Mem.load_store_same; eauto.
+
+        unfold Cop.sem_mod.
+        unfold Cop.sem_binarith. cbn.
+        unfold Cop.sem_cast. cbn.
+        destruct Archi.ptr64. cbn.
+        rewrite Int.eq_false. reflexivity.
+        intros contra. assert (Int.unsigned (Int.repr Nz) = 0).
+        rewrite contra. rewrite Int.unsigned_zero. reflexivity.
+        rewrite Int.unsigned_repr in H1. easy.
+        unfold Nz in *. lia.
+        rewrite Int.eq_false. reflexivity.
+        intros contra. assert (Int.unsigned (Int.repr Nz) = 0).
+        rewrite contra. rewrite Int.unsigned_zero. reflexivity.
+        rewrite Int.unsigned_repr in H1. easy.
+        unfold Nz in *. lia.
+
+        now constructor.
+        crush_star. now constructor.
+      }
+      rewrite lts_spec_step. rewrite !Sup.mor_join. apply join_r.
+      unfold fsup. rewrite !Sup.mor. eapply (sup_at (exist _ _ _)); cbn.
+      Unshelve. 3: { cbn. econstructor. } cbn.
+      (* re-establish the relation *)
+      setoid_rewrite FCD.ext_ana. cbn.
+      setoid_rewrite FCD.ext_ana. cbn.
+      rewrite !Sup.mor.
+      eapply (sup_at (exist _ (Vint i, m'') _)); cbn. Unshelve.
+      2: { cbn. apply HRc. reflexivity. } cbn.
+      setoid_rewrite FCD.ext_ana. cbn.
+      eapply (sup_at (exist _ (c1, (f, (S c1 mod CAL.N)%nat, c2)) _)); cbn.
+      Unshelve.
+      2: {
+        cbn. apply HRp. split; eauto.
+        - apply HR1. cbn. now constructor.
+        - apply HRx. cbn. constructor; eauto.
+          + econstructor; eauto.
+            * erewrite Mem.load_store_same; eauto.
+            * cbn. constructor.
+              apply cnt_inc_simp; assumption.
+            * apply Nat.mod_upper_bound. lia.
+            * intros ofs Hofs. eapply Mem.perm_store_1; eauto.
+              eapply Mem.perm_store_1; eauto.
+          + inv H3. econstructor; eauto.
+            * assert (b1 <> b0).
+              { intros <-. exploit Genv.find_symbol_injective.
+                apply H. apply H1. easy. }
+              erewrite Mem.load_store_other. 2: apply Hm''. 2: left; auto.
+              erewrite Mem.load_store_other; eauto.
+            * intros ofs Hofs. eapply Mem.perm_store_1; eauto.
+              eapply Mem.perm_store_1; eauto.
+          + inv H5. assert (b0 <> b1).
+            { intros <-. exploit Genv.find_symbol_injective.
+              apply H. apply H1. easy. }
+            econstructor; eauto.
+            * intros ix. edestruct (H8 ix) as (vx & Hvx & Hrx).
+              exists vx. split; eauto.
+              erewrite Mem.load_store_other. 2: apply Hm''. 2: left; auto.
+              erewrite Mem.load_store_other; eauto.
+            * intros ofs Hofs. eapply Mem.perm_store_1; eauto.
+              eapply Mem.perm_store_1; eauto.
+          + erewrite Mem.nextblock_store. 2: apply Hm''.
+            erewrite Mem.nextblock_store; eauto.
+      }
+      reflexivity.
+    (* inc2 *)
+    - clear H5. inv H6.
+      rename H0 into Hb. rename H1 into HR1.
+      setoid_rewrite sup_sup. rewrite !Sup.mor.
+      (* initial_state *)
+      eapply (sup_at (exist _ _ _)); cbn. Unshelve.
+      3: { cbn. repeat econstructor; eauto. inv HRst; eauto. }
+      rewrite lts_spec_step.
+      rewrite !Sup.mor_join. apply join_l. apply join_l.
+      unfold fsup. rewrite !Sup.mor.
+      inv HRst. inv H3.
+      (* internal steps *)
+      inv H1. rename mm into m.
+      edestruct (Mem.valid_access_store m Mint32 b0 0) as (m' & Hm').
+      {
+        constructor.
+        - intros ofs Hofs. apply H7. cbn [size_chunk] in Hofs. lia.
+        - apply Z.divide_0_r.
+      }
+      edestruct (Mem.valid_access_store m' Mint32 b0 0) as (m'' & Hm'').
+      {
+        constructor.
+        - intros ofs Hofs. eapply Mem.perm_store_1; eauto.
+        - apply Z.divide_0_r.
+      }
+      eapply (sup_at (exist _ _ _)); cbn. Unshelve.
+      5: {
+        cbn.
+        do 7 (lts_step; [ crush_step; crush_expr | ]). now constructor.
+        do 2 (lts_step; [ crush_step; crush_expr | ]). erewrite Mem.load_store_same; eauto.
+
+        unfold Cop.sem_mod.
+        unfold Cop.sem_binarith. cbn.
+        unfold Cop.sem_cast. cbn.
+        destruct Archi.ptr64. cbn.
+        rewrite Int.eq_false. reflexivity.
+        intros contra. assert (Int.unsigned (Int.repr Nz) = 0).
+        rewrite contra. rewrite Int.unsigned_zero. reflexivity.
+        rewrite Int.unsigned_repr in H1. easy.
+        unfold Nz in *. lia.
+        rewrite Int.eq_false. reflexivity.
+        intros contra. assert (Int.unsigned (Int.repr Nz) = 0).
+        rewrite contra. rewrite Int.unsigned_zero. reflexivity.
+        rewrite Int.unsigned_repr in H1. easy.
+        unfold Nz in *. lia.
+
+        now constructor.
+        crush_star. now constructor.
+      }
+      rewrite lts_spec_step. rewrite !Sup.mor_join. apply join_r.
+      unfold fsup. rewrite !Sup.mor. eapply (sup_at (exist _ _ _)); cbn.
+      Unshelve. 3: { cbn. econstructor. } cbn.
+      (* re-establish the relation *)
+      setoid_rewrite FCD.ext_ana. cbn.
+      setoid_rewrite FCD.ext_ana. cbn.
+      rewrite !Sup.mor.
+      eapply (sup_at (exist _ (Vint i, m'') _)); cbn. Unshelve.
+      2: { cbn. apply HRc. reflexivity. } cbn.
+      setoid_rewrite FCD.ext_ana. cbn.
+      eapply (sup_at (exist _ (c2, (f, c1, (S c2 mod CAL.N)%nat)) _)); cbn.
+      Unshelve.
+      2: {
+        cbn. apply HRp. split; eauto.
+        - apply HR1. cbn. now constructor.
+        - apply HRx. cbn. constructor; eauto.
+          + inv H2. econstructor; eauto.
+            * assert (b1 <> b0).
+              { intros <-. exploit Genv.find_symbol_injective.
+                apply H. apply H1. easy. }
+              erewrite Mem.load_store_other. 2: apply Hm''. 2: left; auto.
+              erewrite Mem.load_store_other; eauto.
+            * intros ofs Hofs. eapply Mem.perm_store_1; eauto.
+              eapply Mem.perm_store_1; eauto.
+          + econstructor; eauto.
+            * erewrite Mem.load_store_same; eauto.
+            * cbn. constructor.
+              apply cnt_inc_simp; assumption.
+            * apply Nat.mod_upper_bound. lia.
+            * intros ofs Hofs. eapply Mem.perm_store_1; eauto.
+              eapply Mem.perm_store_1; eauto.
+          + inv H5. assert (b0 <> b1).
+            { intros <-. exploit Genv.find_symbol_injective.
+              apply H. apply H1. easy. }
+            econstructor; eauto.
+            * intros ix. edestruct (H8 ix) as (vx & Hvx & Hrx).
+              exists vx. split; eauto.
+              erewrite Mem.load_store_other. 2: apply Hm''. 2: left; auto.
+              erewrite Mem.load_store_other; eauto.
+            * intros ofs Hofs. eapply Mem.perm_store_1; eauto.
+              eapply Mem.perm_store_1; eauto.
+          + erewrite Mem.nextblock_store. 2: apply Hm''.
+            erewrite Mem.nextblock_store; eauto.
+      }
+      reflexivity.
+  Qed.
+
+End RB.
+
+Section BQ.
+  Context (se: Genv.symtbl).
+
+  Lemma find_enq b:
+    Genv.find_symbol se enq_id = Some b ->
+    Genv.find_funct (Clight.globalenv se bq_program) (Vptr b zero) = Some (Internal bq_enq).
+  Proof. intros. eapply genv_funct_symbol; eauto. Qed.
+
+  Lemma find_deq b:
+    Genv.find_symbol se deq_id = Some b ->
+    Genv.find_funct (Clight.globalenv se bq_program) (Vptr b zero) = Some (Internal bq_deq).
+  Proof. intros. eapply genv_funct_symbol; eauto. Qed.
+
+  Hint Resolve find_enq find_deq.
+
+  Context (Hse: Genv.valid_for (erase_program bq_program) se).
+
+  Lemma inc2_block:
+    exists b, Genv.find_symbol (globalenv ((semantics2 bq_program) se)) inc2_id = Some b /\
+           Genv.find_funct (globalenv ((semantics2 bq_program) se)) (Vptr b zero) = Some inc2_ext.
+  Proof.
+    eapply Genv.find_def_symbol with (id := inc2_id) in Hse .
+    edestruct (proj1 Hse) as (b & Hb1 & Hb2). reflexivity.
+    exists b. split; eauto. eapply genv_funct_symbol; eauto.
+  Qed.
+
+  Lemma set_block:
+    exists b, Genv.find_symbol (globalenv ((semantics2 bq_program) se)) set_id = Some b /\
+           Genv.find_funct (globalenv ((semantics2 bq_program) se)) (Vptr b zero) = Some set_ext.
+  Proof.
+    eapply Genv.find_def_symbol with (id := set_id) in Hse .
+    edestruct (proj1 Hse) as (b & Hb1 & Hb2). reflexivity.
+    exists b. split; eauto. eapply genv_funct_symbol; eauto.
+  Qed.
+
+  Lemma inc1_block:
+    exists b, Genv.find_symbol (globalenv ((semantics2 bq_program) se)) inc1_id = Some b /\
+           Genv.find_funct (globalenv ((semantics2 bq_program) se)) (Vptr b zero) = Some inc1_ext.
+  Proof.
+    eapply Genv.find_def_symbol with (id := inc1_id) in Hse .
+    edestruct (proj1 Hse) as (b & Hb1 & Hb2). reflexivity.
+    exists b. split; eauto. eapply genv_funct_symbol; eauto.
+  Qed.
+
+  Lemma get_block:
+    exists b, Genv.find_symbol (globalenv ((semantics2 bq_program) se)) get_id = Some b /\
+           Genv.find_funct (globalenv ((semantics2 bq_program) se)) (Vptr b zero) = Some get_ext.
+  Proof.
+    eapply Genv.find_def_symbol with (id := get_id) in Hse .
+    edestruct (proj1 Hse) as (b & Hb1 & Hb2). reflexivity.
+    exists b. split; eauto. eapply genv_funct_symbol; eauto.
+  Qed.
+
+  Variable S: Type.
+  Variable R: S -> mem -> Prop.
+
+  Hypothesis R_ple: forall s m, R s m -> Ple (Genv.genv_next se) (Mem.nextblock m).
+  Local Opaque Genv.find_funct.
+
+  Lemma bq_code_correct:
+    slift M_bq [= (right_arrow (bq_rc se * rel_rc R)%rc)
+               @ (right_arrow c_rc)
+               @ ang_lts_spec (semantics2 bq_program se)
+               @ (left_arrow c_rc)
+               @ (left_arrow (rb_rc se * rel_rc R)%rc).
+  Proof.
+    intros ? [? ? m [ s ]]. Local Opaque semantics2.
+    unfold compose. cbn. unfold rc_adj_right. cbn.
+    inf_intro ar. inf_intro x. destruct x as [ ? ? c_m [ mm ] ].
+    destruct c_m as [vf sg args].
+    inf_intro x. destruct x as [ Rp Hr ]. cbn.
+    intm. inf_intro ar'. inf_intro q. destruct q as [ q ].
+    inf_intro x. destruct x as [ Rc Hc ]. cbn.
+    intm. simple inversion Hc. intros. depsubst.
+    inv H3. inv H5. clear Hc H2 H4. rename H1 into HRc.
+    simple inversion Hr.
+    apply type_pair_des in H2. inv H2.
+    apply type_pair_des in H4. inv H4.
+    depsubst. inv H3. inv H5.
+    depsubst. cbn. intros HRev HRst HRp.
+    simple inversion HRst. depsubst. clear H1 H3 Hr. inv H2. inv H4.
+    clear HRst. intros HRst HRx.
+    unfold fsup. setoid_rewrite Sup.mor.
+    setoid_rewrite FCD.ext_ana. cbn.
+    rewrite <- Sup.mor.
+    simple inversion HRev; intros; depsubst; clear HRev.
+
+    (* enq *)
+    - clear H6. inv H7.
+      rename H0 into Hb. rename H1 into Hv. rename H2 into HRr.
+      edestruct inc2_block as (inc2b & Hb1 & Hb2).
+      edestruct set_block as (setb & Hb3 & Hb4).
+      setoid_rewrite sup_sup.
+      rewrite !Sup.mor. eapply (sup_at (exist _ _ _)); cbn.
+      Unshelve.
+      3: { cbn. repeat econstructor; eauto. }
+      rewrite lts_spec_step.
+      rewrite !Sup.mor_join. apply join_l. apply join_l.
+      unfold fsup. rewrite !Sup.mor.
+      eapply (sup_at (exist _ _ _)). cbn.
+      Unshelve.
+      3: { cbn. crush_star. apply star_refl. }
+      (* external call to [inc2] *)
+      rewrite lts_spec_step.
+      rewrite !Sup.mor_join. apply join_l. apply join_r.
+      unfold fsup. rewrite !Sup.mor.
+      eapply (sup_at (exist _ _ _)); cbn.
+      Unshelve.
+      3: { cbn. econstructor. eauto. }
+      unfold query_int.
+      rewrite srun_bind. rewrite srun_int.
+      rewrite apply_bind. rewrite apply_int_r.
+      unfold rc_adj_left.
+      rewrite !Sup.mor. eapply (sup_at _).
+      rewrite !Sup.mor. eapply (sup_at _).
+      unfold fsup. rewrite !Sup.mor. eapply (sup_at (exist _ _ _)). cbn.
+      Unshelve.
+      5: { cbn. constructor; try reflexivity.
+           instantiate (1 := (fun '(r, m) (c_r : c_reply) => c_r = cr r m)).
+           reflexivity. }
+      intm.
+      rewrite !Sup.mor. eapply (sup_at _).
+      rewrite !Sup.mor. eapply (sup_at _).
+      rewrite !Sup.mor. eapply (sup_at (exist _ _ _)). cbn.
+      Unshelve.
+      5: {
+        cbn. econstructor.
+        - eapply rb_inc2_rel; eauto. reflexivity.
+        - constructor. eauto. reflexivity.
+        - reflexivity.
+      }
+      unfold ISpec.int at 2 6.
+      rewrite !Sup.mor. apply sup_iff. intros ons. apply (sup_at ons).
+      destruct ons as [ [ n s' ] | ].
+      2: {
+        setoid_rewrite FCD.ext_ana; cbn.
+        setoid_rewrite FCD.ext_ana; cbn. reflexivity.
+      }
+      setoid_rewrite FCD.ext_ana. cbn. rewrite !Sup.mor_join.
+      apply join_lub.
+      { apply join_l. setoid_rewrite FCD.ext_ana; cbn. reflexivity. }
+      apply join_r.
+      inf_intro x. destruct x as [ [vr m'] Hm']. cbn.
+      inv Hm'. inv H. cbn [fst snd] in *. subst.
+      setoid_rewrite FCD.ext_ana.
+      setoid_rewrite FCD.ext_ana. cbn. apply join_r. rstep.
+      inf_intro x. destruct x as [ r_c Hrc ]. cbn.
+      inv Hrc.
+      setoid_rewrite FCD.ext_ana. cbn.
+      setoid_rewrite FCD.ext_ana. cbn.
+      rewrite !Sup.mor. eapply (sup_at (exist _ _ _)); cbn.
+      Unshelve.
+      3: { cbn. constructor. }
+      (* internal steps before calling [set] *)
+      rewrite lts_spec_step.
+      rewrite !Sup.mor_join. apply join_l. apply join_l.
+      unfold fsup. rewrite !Sup.mor.
+      eapply (sup_at (exist _ _ _)); cbn. Unshelve.
+      3: { cbn. crush_star. now constructor. apply star_refl. }
+      (* external call to [set] *)
+      rewrite lts_spec_step.
+      rewrite !Sup.mor_join. apply join_l. apply join_r.
+      unfold fsup. rewrite !Sup.mor.
+      eapply (sup_at (exist _ _ _)); cbn. Unshelve.
+      3: { cbn. econstructor. eauto. }
+      rewrite srun_int. unfold query_int.
+      intm.
+      rewrite !Sup.mor. eapply (sup_at _).
+      rewrite !Sup.mor. eapply (sup_at _).
+      rewrite !Sup.mor. eapply (sup_at (exist _ _ _)). cbn.
+      Unshelve.
+      5: {
+        cbn. constructor; try reflexivity.
+        instantiate (1 := (fun '(r, m) (c_r : c_reply) => c_r = cr r m)). reflexivity.
+      }
+      intm.
+      rewrite !Sup.mor. eapply (sup_at _).
+      rewrite !Sup.mor. eapply (sup_at _).
+      rewrite !Sup.mor. eapply (sup_at (exist _ _ _)). cbn.
+      Unshelve.
+      5: {
+        cbn. repeat econstructor; try reflexivity; eauto.
+        rewrite H1. rewrite Int.repr_unsigned. reflexivity.
+      }
+      unfold ISpec.int at 1 5. rewrite !Sup.mor.
+      apply sup_iff. intros oret. apply (sup_at oret).
+      destruct oret as [ [? s''] | ].
+      2: {
+        setoid_rewrite FCD.ext_ana. cbn.
+        setoid_rewrite FCD.ext_ana. cbn. reflexivity.
+      }
+      setoid_rewrite FCD.ext_ana. cbn.
+      rewrite Sup.mor_join. apply join_r.
+      inf_intro x. destruct x as [ [rv m''] Hrm ]. cbn.
+      inv Hrm. inv H. cbn [fst snd] in *. subst.
+      setoid_rewrite FCD.ext_ana. cbn.
+      setoid_rewrite FCD.ext_ana. cbn.
+      apply join_r.
+      inf_intro x. destruct x as [ rc Hrc ]. cbn.
+      inv Hrc.
+      setoid_rewrite FCD.ext_ana. cbn.
+      setoid_rewrite FCD.ext_ana. cbn.
+      replace (FCD.emb (pcons (st (set n v) s') (tt, s'') (pret (tt, s''))))
+        with (FCD.ext (fun s => FCD.emb (pcons (st (set n v) s') (tt, s'') s)) (ret (tt, s''))).
+      2: { setoid_rewrite FCD.ext_ana. reflexivity. }
+      rstep.
+      rewrite !Sup.mor. eapply (sup_at (exist _ _ _)); cbn.
+      Unshelve.
+      3: { cbn. constructor. }
+
+      rewrite lts_spec_step. rewrite !Sup.mor_join.
+      apply join_l. apply join_l.
+      unfold fsup. rewrite !Sup.mor. eapply (sup_at (exist _ _ _)); cbn.
+      Unshelve.
+      3: { cbn. crush_star. }
+      (* final state *)
+      rewrite lts_spec_step. rewrite !Sup.mor_join. apply join_r.
+      unfold fsup. rewrite !Sup.mor. eapply (sup_at (exist _ _ _)).
+      cbn. Unshelve.
+      3: { cbn. constructor. }
+      setoid_rewrite FCD.ext_ana. cbn.
+      setoid_rewrite FCD.ext_ana. cbn.
+      rewrite Sup.mor. eapply (sup_at (exist _ (_, _) _)).
+      Unshelve.
+      4: { cbn. apply HRc. reflexivity. }
+      setoid_rewrite FCD.ext_ana. cbn.
+      eapply (sup_at (exist _ (_, _) _)).
+      Unshelve.
+      4: {
+        cbn. apply HRp. split.
+        - apply HRr. constructor.
+        - apply HRx. eauto.
+      }
+      cbn. reflexivity.
+    (* deq *)
+    - clear H5. inv H6.
+      edestruct inc1_block as (inc1b & Hb1 & Hb2).
+      edestruct get_block as (getb & Hb3 & Hb4).
+      (* initial_state *)
+      setoid_rewrite sup_sup.
+      rewrite !Sup.mor. eapply (sup_at (exist _ _ _)); cbn.
+      Unshelve.
+      3: { cbn. repeat econstructor; eauto. }
+      rewrite lts_spec_step.
+      rewrite !Sup.mor_join. apply join_l. apply join_l.
+      unfold fsup. rewrite !Sup.mor.
+      eapply (sup_at (exist _ _ _)). cbn.
+      Unshelve.
+      3: { cbn. crush_star. apply star_refl. }
+      (* external call to [inc1] *)
+      rewrite lts_spec_step.
+      rewrite !Sup.mor_join. apply join_l. apply join_r.
+      unfold fsup. rewrite !Sup.mor.
+      eapply (sup_at (exist _ _ _)); cbn.
+      Unshelve.
+      3: { cbn. econstructor. eauto. }
+      unfold query_int.
+      rewrite srun_bind. rewrite srun_int.
+      rewrite apply_bind. rewrite apply_int_r.
+      unfold rc_adj_left.
+      rewrite !Sup.mor. eapply (sup_at _).
+      rewrite !Sup.mor. eapply (sup_at _).
+      unfold fsup. rewrite !Sup.mor. eapply (sup_at (exist _ _ _)). cbn.
+      Unshelve.
+      5: { cbn. constructor; try reflexivity.
+           instantiate (1 := (fun '(r, m) (c_r : c_reply) => c_r = cr r m)).
+           reflexivity. }
+      intm.
+      rewrite !Sup.mor. eapply (sup_at _).
+      rewrite !Sup.mor. eapply (sup_at _).
+      rewrite !Sup.mor. eapply (sup_at (exist _ _ _)). cbn.
+      Unshelve.
+      5: {
+        cbn. econstructor.
+        - eapply rb_inc1_rel; eauto. reflexivity.
+        - constructor. eauto. reflexivity.
+        - reflexivity.
+      }
+      unfold ISpec.int at 2 6.
+      rewrite !Sup.mor. apply sup_iff. intros ons. apply (sup_at ons).
+      destruct ons as [ [ n s' ] | ].
+      2: {
+        setoid_rewrite FCD.ext_ana; cbn.
+        setoid_rewrite FCD.ext_ana; cbn. reflexivity.
+      }
+      setoid_rewrite FCD.ext_ana. cbn. rewrite !Sup.mor_join.
+      apply join_lub.
+      { apply join_l. setoid_rewrite FCD.ext_ana; cbn. reflexivity. }
+      apply join_r.
+      inf_intro x. destruct x as [ [vr m'] Hm']. cbn.
+      inv Hm'. inv H. cbn [fst snd] in *. subst.
+      setoid_rewrite FCD.ext_ana.
+      setoid_rewrite FCD.ext_ana. cbn. apply join_r. rstep.
+      inf_intro x. destruct x as [ r_c Hrc ]. cbn.
+      inv Hrc.
+      setoid_rewrite FCD.ext_ana. cbn.
+      setoid_rewrite FCD.ext_ana. cbn.
+      rewrite !Sup.mor. eapply (sup_at (exist _ _ _)); cbn.
+      Unshelve.
+      3: { cbn. constructor. }
+      (* internal steps before calling [get] *)
+      rewrite lts_spec_step.
+      rewrite !Sup.mor_join. apply join_l. apply join_l.
+      unfold fsup. rewrite !Sup.mor.
+      eapply (sup_at (exist _ _ _)); cbn. Unshelve.
+      3: { cbn. crush_star. now constructor. apply star_refl. }
+      (* external call to [get] *)
+      rewrite lts_spec_step.
+      rewrite !Sup.mor_join. apply join_l. apply join_r.
+      unfold fsup. rewrite !Sup.mor.
+      eapply (sup_at (exist _ _ _)); cbn. Unshelve.
+      3: { cbn. econstructor. eauto. }
+      rewrite srun_int. unfold query_int.
+      intm.
+      rewrite !Sup.mor. eapply (sup_at _).
+      rewrite !Sup.mor. eapply (sup_at _).
+      rewrite !Sup.mor. eapply (sup_at (exist _ _ _)). cbn.
+      Unshelve.
+      5: {
+        cbn. constructor; try reflexivity.
+        instantiate (1 := (fun '(r, m) (c_r : c_reply) => c_r = cr r m)).
+        reflexivity.
+      }
+      intm.
+      rewrite !Sup.mor. eapply (sup_at _).
+      rewrite !Sup.mor. eapply (sup_at _).
+      rewrite !Sup.mor. eapply (sup_at (exist _ _ _)). cbn.
+      Unshelve.
+      5: {
+        cbn. repeat econstructor; try reflexivity; eauto.
+        rewrite H3. rewrite Int.repr_unsigned. reflexivity.
+      }
+      unfold ISpec.int at 1 5. rewrite !Sup.mor.
+      apply sup_iff. intros oret. apply (sup_at oret).
+      destruct oret as [ [? s''] | ].
+      2: {
+        setoid_rewrite FCD.ext_ana. cbn.
+        setoid_rewrite FCD.ext_ana. cbn. reflexivity.
+      }
+      setoid_rewrite FCD.ext_ana. cbn.
+      rewrite Sup.mor_join. apply join_r.
+      inf_intro x. destruct x as [ [rv m''] Hrm ]. cbn.
+      inv Hrm. cbn [fst snd] in *.
+      setoid_rewrite FCD.ext_ana. cbn.
+      setoid_rewrite FCD.ext_ana. cbn.
+      apply join_r.
+      inf_intro x. destruct x as [ rc Hrc ]. cbn.
+      inv Hrc.
+      setoid_rewrite FCD.ext_ana. cbn.
+      setoid_rewrite FCD.ext_ana. cbn.
+      replace (FCD.emb (pcons (st (CAL.get n) s') (v, s'') (pret (v, s''))))
+        with (FCD.ext (fun s => FCD.emb (pcons (st (CAL.get n) s') (v, s'') s)) (ret (v, s''))).
+      2: { setoid_rewrite FCD.ext_ana. reflexivity. }
+      rstep.
+      rewrite !Sup.mor. eapply (sup_at (exist _ _ _)); cbn.
+      Unshelve.
+      3: { cbn. constructor. }
+
+      rewrite lts_spec_step. rewrite !Sup.mor_join.
+      apply join_l. apply join_l.
+      unfold fsup. rewrite !Sup.mor. eapply (sup_at (exist _ _ _)); cbn.
+      Unshelve.
+      3: { cbn. crush_star. }
+      (* final state *)
+      rewrite lts_spec_step. rewrite !Sup.mor_join. apply join_r.
+      unfold fsup. rewrite !Sup.mor. eapply (sup_at (exist _ _ _)).
+      cbn. Unshelve.
+      3: { cbn. constructor. }
+      setoid_rewrite FCD.ext_ana. cbn.
+      setoid_rewrite FCD.ext_ana. cbn.
+      rewrite Sup.mor. eapply (sup_at (exist _ (_, _) _)).
+      Unshelve.
+      4: { cbn. apply HRc. reflexivity. }
+      setoid_rewrite FCD.ext_ana. cbn.
+      eapply (sup_at (exist _ (_, _) _)).
+      Unshelve.
+      4: {
+        cbn. apply HRp. split.
+        - apply H1. cbn. eauto.
+        - apply HRx. eauto.
+      }
+      cbn. reflexivity.
+  Qed.
+
+End BQ.
+
+Section COMPOSITION.
+
+  Context (se: Genv.symtbl).
+  Context {L} (COMP: CategoricalComp.comp_semantics
+                       (semantics2 bq_program)
+                       (semantics2 rb_program) = Some L).
+
+  Lemma rb_bq_code_correct:
+    slift M_bq @ L_rb [= right_arrow (bq_rc se * rel_rc (R_rb se))%rc
+                      @ right_arrow c_rc
+                      @ ang_lts_spec (L se)
+                      @ bot.
+  Proof.
+    rewrite bq_code_correct by admit.
+    rewrite rb_code_correct by admit.
+    rewrite !compose_assoc.
+    rewrite <- (compose_assoc _ (right_arrow _) (left_arrow _)).
+    rewrite epsilon. rewrite compose_unit_l.
+    rewrite <- (compose_assoc _ (right_arrow _) (left_arrow _)).
+    rewrite epsilon. rewrite compose_unit_l.
+    rewrite <- (compose_assoc _ (ang_lts_spec _) (ang_lts_spec _)).
+    rewrite comp_embed by apply COMP. reflexivity.
+  Admitted.
+
+End COMPOSITION.
